A model with f : nat -> nat. Fundamental Lemma is proven.

theories/LContexts.v
@@ -3,9 +3,9 @@ Require Import Coq.Arith.EqNat PeanoNat.
 From LogRel.AutoSubst Require Import core unscoped Ast Extra.
 From LogRel Require Import Utils.
 
-Notation LCon := (list (prod nat bool)).
+Notation LCon := (list (prod nat nat)).
 
-Inductive in_LCon : LCon -> nat -> bool -> SProp :=
+Inductive in_LCon : LCon -> nat -> nat -> SProp :=
 | in_here_l (l : LCon) {n b} : in_LCon (cons (n,b) l) n b
 | in_there_l {l : LCon} {n b d} : in_LCon l n b -> in_LCon (cons d l) n b.
 
@@ -87,34 +87,24 @@ Qed.
 Lemma uniqueinLCon {l n b b'} : wf_LCon l -> in_LCon l n b -> in_LCon l n b' -> b = b'.
 Proof.
   intros wfl inl inl'.
-  destruct b ; destruct b' ; auto.
-  all: enough (H : SFalse) by inversion H.
-  - revert inl inl' ; induction wfl ; intros.
-    + now inversion inl.
-    + inversion inl ; subst.
-      * inversion inl' ; subst ; trivial.
-        exfalso.
-        exact (notinLConnotinLCon n1 H3).
-      * inversion inl' ; subst.
-        -- exfalso ; exact (notinLConnotinLCon n1 H3).
-        -- exact (IHwfl H3 H4).
-  - revert inl inl' ; induction wfl ; intros.
-    + now inversion inl.
-    + inversion inl ; subst.
-      * inversion inl' ; subst ; trivial.
-        exfalso.
-        exact (notinLConnotinLCon n1 H3).
-      * inversion inl' ; subst.
-        -- exfalso ; exact (notinLConnotinLCon n1 H3).
-        -- exact (IHwfl H3 H4).
+  destruct (Nat.eq_dec b b') ; [assumption | ].
+  enough (H : SFalse) by inversion H.
+  revert inl inl' ; induction wfl ; intros.
+  - now inversion inl.
+  - inversion inl ; subst.
+    + inversion inl' ; subst ; trivial.
+      1: exfalso ; now eapply n0.
+      exfalso.
+      exact (notinLConnotinLCon n2 H3).
+    + inversion inl' ; subst.
+      * exfalso ; exact (notinLConnotinLCon n2 H3).
+      * exact (IHwfl H3 H4).
 Qed.
 
 Inductive or_inLCon l n : Type :=
-| or_inltrue : in_LCon l n true -> or_inLCon l n
-| or_inlfalse : in_LCon l n false -> or_inLCon l n
+| or_inl : forall m, in_LCon l n m  -> or_inLCon l n
 | or_notinl : not_in_LCon l n -> or_inLCon l n.
-Arguments or_inltrue [_ _] _.
-Arguments or_inlfalse [_ _] _.
+Arguments or_inl [_ _] _.
 Arguments or_notinl [_ _] _.
 
 Fixpoint decidInLCon l n : or_inLCon l n .
@@ -123,47 +113,30 @@ Proof.
                    | nil => _
                    | cons (m, b) q => _
                    end).
-  - econstructor 3 ; now econstructor.
+  - econstructor 2 ; now econstructor.
   - unshelve refine
       (match (decidInLCon q n) with
-       | or_inltrue H => _
-       | or_inlfalse H => _ 
+       | or_inl m H => _
        | or_notinl H => _
        end).
     + econstructor 1. now econstructor.
-    + econstructor 2 ; now econstructor.
     + case (eq_nat_decide n m).
       * intro neqm.
         rewrite <- (proj1 (eq_nat_is_eq n m) neqm).
-        case b.
-        -- econstructor 1 ; now econstructor.
-        -- econstructor 2 ; now econstructor.
+        econstructor 1 ; now econstructor.
       * intro noteq.
-        econstructor 3.
+        econstructor 2.
         econstructor ; try assumption.
         intro neqm ; rewrite neqm in noteq.
         eapply noteq.
         exact (eq_nat_refl _).
 Defined.
 
-Lemma decidInLCon_true (l : wfLCon) n (Hin: in_LCon l n true) :
-  decidInLCon l n = or_inltrue Hin.
+Lemma decidInLCon_true (l : wfLCon) n m (Hin: in_LCon l n m) :
+  decidInLCon l n = or_inl m Hin.
 Proof.
   destruct (decidInLCon l n).
-  + reflexivity.
-  + exfalso.
-    assert (H := uniqueinLCon l.(pi2) Hin i) ; now inversion H.
-  + exfalso.
-    now eapply notinLConnotinLCon.
-Qed.
-
-Lemma decidInLCon_false (l : wfLCon) n (Hin: in_LCon l n false) :
-  decidInLCon l n = or_inlfalse Hin.
-Proof.
-  destruct (decidInLCon l n).
-  + exfalso.
-    assert (H := uniqueinLCon l.(pi2) Hin i) ; now inversion H.
-  + reflexivity.
+  + assert (H := uniqueinLCon l.(pi2) Hin i) ; now subst. 
   + exfalso.
     now eapply notinLConnotinLCon.
 Qed.
@@ -174,39 +147,14 @@ Proof.
   destruct (decidInLCon l n).
   + exfalso.
     now eapply notinLConnotinLCon.
-  + exfalso.
-    now eapply notinLConnotinLCon.
   + reflexivity. 
 Qed.
 
 Arguments decidInLCon_true [_ _] _.
-Arguments decidInLCon_false [_ _] _.
 Arguments decidInLCon_notinLCon [_ _] _.
 
-(*  induction l.
-  - right.
-    now econstructor.
-  - induction IHl as [IHl | IHl ].
-    + induction IHl as [IHl | IHl].
-      * left ; left ; now econstructor.
-      * left ; right ; now econstructor.
-    + destruct a as [m b].
-      case (eq_nat_decide n m).
-      * intro neqm.
-        rewrite <- (proj1 (eq_nat_is_eq n m) neqm).
-        case b.
-        -- left ; left ; now econstructor.
-        -- left ; right ; now econstructor.
-      * intro noteq.
-        right.
-        econstructor ; try assumption.
-        intro neqm ; rewrite neqm in noteq.
-        eapply noteq.
-        exact (eq_nat_refl _).
-Defined.        *)
-        
       
-Definition wfLCons (l : wfLCon) {n : nat} (ne : not_in_LCon (pi1 l) n) (b : bool) : wfLCon.
+Definition wfLCons (l : wfLCon) {n : nat} (ne : not_in_LCon (pi1 l) n) (b : nat) : wfLCon.
 Proof.
   exists (cons (n,b) (pi1 l)).
   econstructor ; trivial.
@@ -264,304 +212,13 @@ Qed.
 Lemma not_in_LCon_le_not_in_LCon {l l' n} (ne : not_in_LCon (pi1 l') n) :
   l' ≤ε l -> not_in_LCon (pi1 l) n.
 Proof.
-  intros f ; destruct (decidInLCon l n) as [i | i | ] ; [.. | assumption].
-  1,2: exfalso ; eapply notinLConnotinLCon ; eauto.
+  intros f ; destruct (decidInLCon l n) as [i | ] ; [.. | assumption].
+  1: exfalso ; eapply notinLConnotinLCon ; eauto.
 Qed.
 
-
-Definition AllInLCon (n : nat) (l : wfLCon) : SProp :=
-  forall (m : nat), m < n -> Sor (in_LCon l m true) (in_LCon l m false).
-
-
-
-Lemma AllInLCon_le (n m : nat) (ninfm : n <= m) (l : wfLCon) :
-  AllInLCon m l -> AllInLCon n l.
-Proof.
-  intros allinl k kinfm.
-  unshelve refine (allinl k _).
-  now eapply Nat.lt_le_trans.
-Qed.
-
-Lemma AllInLCon_S (n : nat) b l :
-  AllInLCon n l -> in_LCon l n b -> AllInLCon (S n) l.
-Proof.
-  intros allinl ninl m minfSn.
-  case (Compare_dec.le_lt_eq_dec m n).
-  - now eapply PeanoNat.lt_n_Sm_le.
-  - intro minfn ; clear minfSn.
-    now eapply allinl.
-  - intro eq ; subst.
-    destruct b.
-    + now left.
-    + now right.
-      
-Qed.
-  
-
-Fixpoint Lack_n (l : wfLCon) (n : nat) : list nat :=
-  match n with
-  | 0 => nil
-  | S k => match decidInLCon l k with
-             | or_notinl H => cons k (Lack_n l k)
-             | _ =>  Lack_n l k
-             end
-  end.
-
-Fixpoint In {A : Type} (a : A) (l : list A) {struct l} : Type :=
-  match l with
-  | nil => False
-  | (b :: m)%list => (b = a) + In a m
-  end.
-
-Definition Incl {A : Type} (l l' : list A) : Type :=
-  forall a : A, In a l -> In a l'.
-
-Lemma Incl_nil {A} : forall (l : list A), Incl l nil -> l = nil.
-Proof.
-  intros.
-  induction l.
-  - reflexivity.
-  - pose proof (t := X a (inl (eq_refl _))).
-    now inversion t.
-Qed.
-  
-Lemma Lack_n_notinLCon (n m : nat) (l : wfLCon) :
-  In m (Lack_n l n) -> not_in_LCon l m.
-Proof.
-  revert m l.
-  induction n.
-  - intros.
-    now exfalso.
-  - intros.
-    unfold Lack_n in X.
-    destruct (decidInLCon l n) ; fold Lack_n in X.
-    + cbn in *.
-      now eapply IHn.
-    + cbn in *.
-      now eapply IHn.
-    + destruct X.
-      * now rewrite <- e.
-      * now eapply IHn.
-Qed.
-
-Lemma Lack_n_minfn (n m : nat) (l : wfLCon) :
-  In m (Lack_n l n) -> m < n.
-Proof.
-  induction n.
-  - intros ; exfalso.
-    now inversion X.
-  - intro inm.
-    cbn in *.
-    destruct (decidInLCon l n).
-    + etransitivity.
-      now eapply IHn.
-      now eapply Nat.lt_succ_diag_r.
-    + etransitivity.
-      now eapply IHn.
-      now eapply Nat.lt_succ_diag_r.
-    + cbn in inm.
-      destruct inm.
-      * rewrite e.
-        now eapply Nat.lt_succ_diag_r.
-      * etransitivity.
-        now eapply IHn.
-        now eapply Nat.lt_succ_diag_r.
-Qed.
-
-
-Lemma notinLCon_Lack_n (n m : nat) (l : wfLCon) :
-  m < n -> not_in_LCon l m -> In m (Lack_n l n).
-Proof.
-  induction n.
-  - intros ; simpl.
-    now inversion H.
-  - intros ; simpl.
-    destruct (Compare_dec.le_lt_eq_dec _ _  H).
-    + eapply Arith_base.lt_S_n_stt in l0.
-      destruct (decidInLCon l n).
-      * now eapply IHn.
-      * now eapply IHn.
-      * right.
-        now eapply IHn.
-    + injection e ; intros ; subst ; clear e.
-      destruct (decidInLCon l n).
-      * exfalso.
-        now eapply notinLConnotinLCon.
-      * exfalso.
-        now eapply notinLConnotinLCon.
-      * left ; reflexivity.
-Qed.
-      
-  
-Lemma Lack_n_Lcon_le (n : nat) (l l' : wfLCon) :
-  l' ≤ε l -> Incl (Lack_n l' n) (Lack_n l n).
-Proof.
-  intros f.
-  induction n ; intros m inm.
-  - now exfalso.
-  - pose proof (Lack_n_minfn _ _ _ inm) as minfSn.
-    pose proof (notinl' := Lack_n_notinLCon _ _ _ inm).
-    eapply notinLCon_Lack_n ; try eassumption.
-    destruct (decidInLCon l m) ; try assumption.
-    all: exfalso ; eapply notinLConnotinLCon ; try eassumption.
-    all: now eapply f.
-Qed.
-
-Lemma Lack_n_le (n m : nat) (l : wfLCon) :
-  n <= m -> Incl (Lack_n l n) (Lack_n l m).
-Proof.
-  intro ninfm.
-  induction n.
-  - intros k ink.
-    inversion ink.
-  - cbn.
-    destruct (decidInLCon l n).
-    + now eapply IHn, Nat.lt_le_incl, (proj1 (Nat.le_succ_l n m)).
-    + now eapply IHn, Nat.lt_le_incl, (proj1 (Nat.le_succ_l n m)).
-    + intros k ink.
-      destruct ink.
-      * subst.
-        eapply notinLCon_Lack_n ; try assumption.
-      * eapply IHn ; try assumption.
-        now eapply Nat.lt_le_incl, (proj1 (Nat.le_succ_l n m)).
-Qed.
 
 
     
-
-Lemma Lack_n_Sn_eq (n m : nat) (l : wfLCon) (q : list nat) :
-  Lack_n l (S n) = cons m q -> not_in_LCon l n ->  n = m.
-Proof.
-  revert m.
-  induction n ; intros m Heq notinl.
-  - cbn in *.
-    destruct (decidInLCon l 0).
-    + exfalso ; now inversion Heq.
-    + exfalso ; now inversion Heq.
-    + now inversion Heq.
-  - cbn in *.
-    destruct (decidInLCon l (S n)).
-    + exfalso ; eapply notinLConnotinLCon ; eassumption.
-    + exfalso ; eapply notinLConnotinLCon ; eassumption.
-    + now inversion Heq.
-Qed.
-
-  
-Lemma Lack_n_add (n m : nat) (l : wfLCon) (me : not_in_LCon l m)
-  (q : list nat) (b : bool) :
-  cons m q = Lack_n l n -> Lack_n (l ,,l (me, b)) n = q.
-Proof.
-  intros Heq.
-  unfold Lack_n.
-  revert q m me Heq.
-  induction n ; intros.
-  - exfalso.
-    now inversion Heq.
-  - fold Lack_n in *.
-    pose proof (t:= Lack_n_Sn_eq _ _ _ _ (eq_sym Heq)).
-    destruct l as [l wfl].
-    cbn in *.
-    remember (decidInLCon l n) as rem.
-    destruct rem as [ s | s | s].
-    + cbn in *.
-      subst. now eapply IHn.
-    + subst. now eapply IHn.
-    + assert (forall (m : nat) (e : m = m), e = eq_refl _).
-      * clear n l wfl b IHn q m me s Heqrem Heq t.
-        refine (fix f m :=
-                  match m as m0 return forall e : m0 = m0, e = eq_refl _ with
-                | 0 => fun e => match e with
-                         | eq_refl _ => eq_refl _
-                       end
-                  | S k => _
-                  end).
-        admit.
-      * pose proof (t' := t s) ; clear t.
-        subst.
-        destruct eq_nat_decide.
-        rewrite (H m (proj1 (eq_nat_is_eq m m) e)).
-        cbn.
-        destruct b.
-        -- eapply IHn.
-Admitted.     
-
-Axiom todo : False.
-  
-Lemma Lack_nil_AllInLCon (n : nat) (l : wfLCon) :
-  Lack_n l n = nil -> AllInLCon n l.
-Proof.
-  induction n.
-  - intros eq0 m minf0.
-    exfalso.
-    now eapply Nat.nle_succ_0. 
-  - intro Hyp ; cbn in *.
-    destruct (decidInLCon l n).
-    + intros m minfn.
-      destruct (Compare_dec.le_lt_eq_dec _ _ minfn) as [ | eqSnm].
-      * apply (IHn Hyp).
-        now apply Arith_base.lt_S_n_stt.
-      * injection eqSnm ; intros eqnm.
-        now subst.
-    + intros m minfn.
-      destruct (Compare_dec.le_lt_eq_dec _ _ minfn) as [ | eqSnm].
-      * apply (IHn Hyp).
-        now apply Arith_base.lt_S_n_stt.
-      * injection eqSnm ; intros eqnm.
-        now subst.
-    + exfalso.
-      now inversion Hyp.
-Qed.
-
-    
-(*Fixpoint RemoveElt {l : LCon} {n b} (ne : in_LCon l n b) : LCon
-  := match ne with
-     | in_here_l l => l
-     | @in_there_l l n b d ne => cons d (RemoveElt ne)
-     end.
-
-Lemma Remove_notinLCon {l : LCon} {n m b} (ne : in_LCon l n b) (me : not_in_LCon l m) :
-  not_in_LCon (RemoveElt ne) m.
-Proof.
-  induction ne.
-  - cbn in *.
-    now inversion me.
-  - destruct d ; cbn in *.
-    inversion me ; subst.
-    econstructor.
-    + assumption.
-    + now apply IHne.
-Qed.
-
-Definition wf_RemoveElt {l : wfLCon} {n b} (ne : in_LCon l n b) : wfLCon.
-Proof.
-  exists (RemoveElt ne).
-  destruct l as [l wfl] ; cbn in *.
-  induction ne.
-  - now inversion wfl.
-  - cbn.
-    destruct d.
-    econstructor.
-    + eapply IHne.
-      now inversion wfl.
-    + eapply Remove_notinLCon.
-      now inversion wfl.
-Defined.
-
-Lemma RemoveElt_le {l l' n b} (f : l' ≤ε l) (ne : in_LCon l n b) :
-  (wf_RemoveElt (f n b ne))  ≤ε (wf_RemoveElt ne).
-Proof.
-Admitted.
-  
-Lemma LCon_le_le {l l'} :  l' ≤ε l -> length l <= length l'.
-Proof.
-  intro f.
-  destruct l as [l wfl] ; cbn in *.
-  revert l' f.
-  induction wfl ; intros.
-  - now eapply le_0_n.
-  -
-Admitted.*)
-
 Fixpoint LCon_newElt (l : LCon) : nat :=
   match l with
   | nil => 0
@@ -590,321 +247,3 @@ Proof.
   pose proof (newElt_newElt_aux l 0).
   now erewrite Nat.max_0_r in H.
 Qed.
-
-Fixpoint Max_Bar_aux
-  (wl : wfLCon) (n : nat) (q : list nat) :
-  forall (e : q = Lack_n wl n)
-         (P : forall wl', wl' ≤ε wl -> AllInLCon n wl' -> nat),
-    nat.
-Proof.
-  revert wl.
-  refine (match q with
-          | nil => _
-          | cons a q => _
-          end) ; intros.
-  - refine (P wl _ _).
-    now eapply (idε).
-    eapply Lack_nil_AllInLCon.
-    now symmetry.
-  - refine (max _ _).
-    + unshelve eapply Max_Bar_aux.
-      * unshelve eapply wfLCons ; [exact wl | exact a | | exact true].
-        eapply Lack_n_notinLCon.
-        rewrite <- e.
-        now left.
-      * exact n.
-      * exact q.
-      * symmetry.
-        now eapply Lack_n_add.
-      * intros * τ allinl.
-        refine (P wl' _ allinl).
-        unshelve eapply (_ •ε _).
-        3: eapply LCon_le_step ; now eapply wfLCon_le_id.
-        eassumption.
-    + unshelve refine (Max_Bar_aux _ n q _ _).
-      * unshelve eapply wfLCons ; [exact wl | exact a | | exact false].
-        eapply Lack_n_notinLCon.
-        rewrite <- e.
-        now left.
-      * symmetry.
-        now eapply Lack_n_add.
-      * intros * τ allinl.
-        refine (P wl' _ allinl).
-        eapply wfLCon_le_trans ; try eassumption.
-        eapply LCon_le_step.
-        now eapply wfLCon_le_id.
-Defined.        
-
-Definition Max_Bar (wl : wfLCon) (n : nat)
-  (P: forall wl' : wfLCon, wl' ≤ε wl -> AllInLCon n wl' -> nat) : nat :=
-  Max_Bar_aux wl n (Lack_n wl n) eq_refl P.
-
-
-(*
-Lemma Max_Bar_aux_le (wl : wfLCon) (n : nat)
-  (q : list nat)
-  (e : q = Lack_n wl n)
-  (P : forall wl' : wfLCon, wl' ≤ε wl -> AllInLCon n wl' -> nat)
-  (Pe : forall (wl' wl'' : wfLCon)
-               (τ : wl' ≤ε wl) (τ' : wl'' ≤ε wl),
-      wl'' ≤ε wl' ->
-      forall (ne : AllInLCon n wl') (ne' : AllInLCon n wl''),
-        P wl'' τ' ne' <= P wl' τ ne)
-  (wl' : wfLCon) (τ : wl' ≤ε wl) (ne : AllInLCon n wl') :
-  P wl' τ ne <= Max_Bar_aux wl n q e P.
-Proof.
-  revert wl wl' ne e τ P Pe.
-  induction q ; intros.
-  - cbn.
-    now eapply Pe.
-  - cbn.
-    edestruct (ne a).
-    + unshelve eapply Lack_n_minfn.
-      exact wl.
-      rewrite <- e.
-      now left.
-    + etransitivity.
-      2: now eapply Nat.max_lub_l.
-      etransitivity.
-      2:{ unshelve eapply IHq.
-          * exact wl'.
-          * eapply LCon_le_in_LCon ; eassumption. 
-          * assumption.
-          * intros.
-            now eapply Pe.
-      }
-      eapply Pe.
-      now eapply wfLCon_le_id.
-    + etransitivity.
-      2: now eapply Nat.max_lub_r.
-      etransitivity.
-      2:{ unshelve eapply IHq.
-          * exact wl'.
-          * eapply LCon_le_in_LCon ; eassumption. 
-          * assumption.
-          * intros.
-            now eapply Pe.
-      }
-      eapply Pe.
-      now eapply wfLCon_le_id.
-Qed.
-
-Lemma Max_Bar_le (wl : wfLCon) (n : nat)
-  (P : forall wl' : wfLCon, wl' ≤ε wl -> AllInLCon n wl' -> nat)
-  (Pe : forall (wl' wl'' : wfLCon)
-               (τ : wl' ≤ε wl) (τ' : wl'' ≤ε wl),
-      wl'' ≤ε wl' ->
-      forall (ne : AllInLCon n wl') (ne' : AllInLCon n wl''),
-        P wl'' τ' ne' <= P wl' τ ne)
-  (wl' : wfLCon) (τ : wl' ≤ε wl) (ne : AllInLCon n wl') :
-  P wl' τ ne <= Max_Bar wl n P.
-Proof.
-  unfold Max_Bar.
-  now eapply Max_Bar_aux_le.
-Qed.
-
-Fixpoint Bar_lub_aux (wl wl' : wfLCon) (n : nat) (f : wl' ≤ε wl)
-         (Hyp : AllInLCon n wl')
-         (q : list nat) :
-  forall (e : q = Lack_n wl n), wfLCon.
-Proof.
-  refine (match q with
-          | nil => _
-          | cons a q' => _
-          end).
-  - exact (fun _ => wl).
-  - intros e.
-    assert (a < n).
-    abstract (refine (Lack_n_minfn _ _ _ _) ;
-              erewrite <- e ;
-              now left).
-    destruct (Hyp a H).
-    + unshelve eapply Bar_lub_aux.
-      * refine (wfLCons _ _ true).
-        eapply Lack_n_notinLCon.
-        erewrite <- e.
-        now left.
-      * exact wl'.
-      * exact n.
-      * exact q'.
-      * now eapply LCon_le_in_LCon.
-      * assumption.
-      * symmetry.
-        now eapply Lack_n_add.
-    + unshelve eapply Bar_lub_aux.
-      * refine (wfLCons _ _ false).
-        eapply Lack_n_notinLCon.
-        erewrite <- e.
-        now left.
-      * exact wl'.
-      * exact n.
-      * exact q'.
-      * now eapply LCon_le_in_LCon.
-      * assumption.
-      * symmetry.
-        now eapply Lack_n_add.
-Defined.
-
-Definition Bar_lub (wl wl' : wfLCon) (n : nat) (f : wl' ≤ε wl)
-  (Hyp : AllInLCon n wl') : wfLCon.
-Proof.
-  eapply Bar_lub_aux ; try eassumption.
-  reflexivity.
-Defined.
-
-Lemma Bar_lub_eq (wl wl' wl'' : wfLCon) (n : nat)
-  (f : wl' ≤ε wl) (f' : wl'' ≤ε wl) (f'': wl'' ≤ε wl')
-  (Hyp : AllInLCon n wl') (Hyp' : AllInLCon n wl'')
-  (q : list nat) (e : q = Lack_n wl n) :
-  (Bar_lub_aux wl wl'' n f' Hyp' q e) = (Bar_lub_aux wl wl' n f Hyp q e).
-Proof.
-  revert wl wl' wl'' f f' f'' Hyp Hyp' e.
-  induction q ; intros.
-  - reflexivity.
-  - cbn.
-    destruct (Hyp' a (Bar_lub_aux_subproof wl n a q e)). 
-    + destruct (Hyp a (Bar_lub_aux_subproof wl n a q e)).
-      * now eapply IHq.
-      * exfalso.
-        change (match true with | true => False | _ => True end).
-        erewrite (uniqueinLCon _ i).
-        2: now eapply f''.
-        easy.
-    + destruct (Hyp a (Bar_lub_aux_subproof wl n a q e)).
-      * exfalso.
-        change (match true with | true => False | _ => True end).
-        erewrite <- (uniqueinLCon _ i).
-        2: now eapply f''.
-        easy.
-      * now eapply IHq.
-        Unshelve.
-        all: now destruct wl''.
-Qed.
-
-
-
-Lemma Bar_lub_smaller_aux (wl wl' : wfLCon) (n : nat) (f : wl' ≤ε wl)
-  (Hyp : AllInLCon n wl') (q : list nat) (e : q = Lack_n wl n):
-  wl' ≤ε (Bar_lub_aux wl wl' n f Hyp q e).
-Proof.
-  revert wl f e.
-  induction q ; intros.
-  - assumption.
-  - cbn.
-    destruct (Hyp a (Bar_lub_aux_subproof wl n a q e)).
-    + now eapply IHq.
-    + now eapply IHq.
-Qed.
-
-Lemma Bar_lub_smaller (wl wl' : wfLCon) (n : nat) (f : wl' ≤ε wl)
-  (Hyp : AllInLCon n wl') :
-  wl' ≤ε (Bar_lub wl wl' n f Hyp).
-Proof.
-  unfold Bar_lub ; eapply Bar_lub_smaller_aux.
-Qed.
-
-
-Lemma Bar_lub_ub_aux (wl wl' : wfLCon) (n : nat) (f : wl' ≤ε wl)
-  (Hyp : AllInLCon n wl') (q : list nat) (e : q = Lack_n wl n) :
-  (Bar_lub_aux wl wl' n f Hyp q e) ≤ε wl.
-Proof.
-  revert wl f e.
-  induction q ; intros.
-  - now eapply wfLCon_le_id.
-  - cbn.
-    destruct (Hyp a (Bar_lub_aux_subproof wl n a q e)).
-    + eapply wfLCon_le_trans.
-      eapply IHq.
-      eapply LCon_le_step.
-      now eapply wfLCon_le_id.
-    + eapply wfLCon_le_trans.
-      eapply IHq.
-      eapply LCon_le_step.
-      now eapply wfLCon_le_id.
-Qed.
-
-Lemma Bar_lub_ub (wl wl' : wfLCon) (n : nat) (f : wl' ≤ε wl)
-  (Hyp : AllInLCon n wl') :
-  (Bar_lub wl wl' n f Hyp) ≤ε wl.
-Proof.
-  unfold Bar_lub ; eapply Bar_lub_ub_aux.
-Qed.
-  
-Lemma Bar_lub_AllInLCon_aux (wl wl' : wfLCon) (n : nat) (f : wl' ≤ε wl)
-  (Hyp : AllInLCon n wl') (q : list nat) (e : q = Lack_n wl n) :
-  AllInLCon n (Bar_lub_aux wl wl' n f Hyp q e).
-Proof.
-  revert wl f e.
-  induction q ; intros.
-  - cbn.
-    now eapply Lack_nil_AllInLCon.
-  - cbn.
-    destruct (Hyp a (Bar_lub_aux_subproof wl n a q e)).
-    + now eapply IHq.
-    + now eapply IHq.
-Qed.
-
-Lemma Bar_lub_AllInLCon
-  (wl wl' : wfLCon) (n : nat) (f : wl' ≤ε wl)
-  (Hyp : AllInLCon n wl') :
-  AllInLCon n (Bar_lub wl wl' n f Hyp).
-Proof.
-  unfold Bar_lub ; eapply Bar_lub_AllInLCon_aux.
-Qed.
-
-
-Lemma Max_Bar_Bar_lub_aux (wl : wfLCon) (n : nat)
-  (P : forall wl' : wfLCon, wl' ≤ε wl -> AllInLCon n wl' -> nat)
-  (wl' : wfLCon) (τ : wl' ≤ε wl) (ne : AllInLCon n wl')
-   q e f allinBar_lub :
-  P (Bar_lub_aux wl wl' n τ ne q e) f allinBar_lub <= Max_Bar_aux wl n q e P.
-Proof.
-  revert wl P τ e f allinBar_lub.
-  induction q ; intros.
-  - cbn in *.
-    erewrite (AllInLCon_Irrel _ _ allinBar_lub (Lack_nil_AllInLCon n wl (eq_sym e))).
-    now erewrite (wfLCon_le_Irrel _ _ f (wfLCon_le_id _)).
-  - cbn in *.
-    destruct (ne a (Bar_lub_aux_subproof wl n a q e)).
-    + etransitivity.
-      2: { eapply Nat.max_lub_l.
-           reflexivity.
-      }
-      etransitivity.
-      2:{ unshelve eapply IHq.
-          + now eapply LCon_le_in_LCon.
-          + eapply Bar_lub_ub_aux.
-          + eapply Bar_lub_AllInLCon_aux.
-      }
-      eapply Nat.eq_le_incl.
-      unshelve erewrite (AllInLCon_Irrel _ _ allinBar_lub).
-      2: erewrite (wfLCon_le_Irrel _ _ f).
-      2: reflexivity.
-    + etransitivity.
-      2: { eapply Nat.max_lub_r.
-           reflexivity.
-      }
-      etransitivity.
-      2:{ unshelve eapply IHq.
-          + now eapply LCon_le_in_LCon.
-          + eapply Bar_lub_ub_aux.
-          + eapply Bar_lub_AllInLCon_aux.
-      }
-      eapply Nat.eq_le_incl.
-      erewrite (AllInLCon_Irrel _ _ allinBar_lub).
-      erewrite (wfLCon_le_Irrel _ _ f).
-      reflexivity.
-Qed.      
-
-Lemma Max_Bar_Bar_lub (wl : wfLCon) (n : nat)
-  (P : forall wl' : wfLCon, wl' ≤ε wl -> AllInLCon n wl' -> nat)
-  (wl' : wfLCon) (τ : wl' ≤ε wl) (ne : AllInLCon n wl')
-  (f : Bar_lub wl wl' n τ ne ≤ε wl)
-  (allinBar : AllInLCon n (Bar_lub wl wl' n τ ne)) :
-  P (Bar_lub wl wl' n τ ne) f allinBar <= Max_Bar wl n P.
-Proof.
-  unfold Bar_lub ; unfold Max_Bar ; cbn.
-  now eapply Max_Bar_Bar_lub_aux.
-Qed.
-
-*)
