theories/Substitution/Split.v
@@ -10,30 +10,18 @@ Section Split.
 Context `{GenericTypingProperties}.
 
 Lemma validTySplit {wl : wfLCon} {Γ l A} {n : nat} {ne : not_in_LCon wl n}
-  {VΓt : [||-v Γ ]< (wl ,,l (ne, true)) >}
-  {VΓf : [||-v Γ ]< (wl ,,l (ne, false)) >}
+  {VΓt : forall m, [||-v Γ ]< (wl ,,l (ne, m)) >}
   {VΓ : [||-v Γ]< wl >} :
-  [Γ ||-v<l> A | VΓt]< wl ,,l (ne, true) > ->
-  [Γ ||-v<l> A | VΓf]< wl ,,l (ne, false) > ->
+  (forall m, [Γ ||-v<l> A | VΓt m]< wl ,,l (ne, m) >) ->
   [Γ ||-v<l> A | VΓ]< wl >.
 Proof.
-  intros [VAt VAextt] [VAf VAextf].
+  intros VAt.
   unshelve econstructor.
   - intros ??????.
-    destruct (decidInLCon wl' n) as [ i | i | notin].
+    destruct (decidInLCon wl' n) as [ m i | notin].
     + pose (f' := LCon_le_in_LCon (ne := ne) f i).
-      pose (f'':= @LCon_le_step wl wl n true ne (wfLCon_le_id _)).
+      pose (f'':= @LCon_le_step wl wl n m ne (wfLCon_le_id _)).
       unshelve eapply VAt ; tea.
-      change f with (f' •ε f'') in vσ.
-      eapply subst_Ltrans' in vσ.
-      unshelve eapply irrelevanceSubst.
-      * exists (VPack_Ltrans f'' VΓ).
-        now eapply  WfC_Ltrans.
-      * assumption.
-      * exact vσ.
-    + pose (f' := LCon_le_in_LCon (ne := ne) f i).
-      pose (f'':= @LCon_le_step wl wl n false ne (wfLCon_le_id _)).
-      unshelve eapply VAf ; tea.
       change f with (f' •ε f'') in vσ.
       eapply subst_Ltrans' in vσ.
       unshelve eapply irrelevanceSubst.
@@ -43,57 +31,31 @@ Proof.
       * exact vσ.
     + unshelve eapply Split.
       2: exact notin.
-      * pose (i := @in_here_l wl' n true).
-        pose (f' := @LCon_le_up wl wl' n true ne notin f). 
-        pose (f'':= @LCon_le_step wl wl n true ne (wfLCon_le_id _)).
-        pose (f''':= @LCon_le_step wl' wl' n true notin (wfLCon_le_id _)).
-        unshelve eapply VAt ; tea.
-        2: unshelve epose proof (X:= subst_Ltrans f''' _ vσ).
-        1,2: now eapply wfc_Ltrans.
-        change (f''' •ε f)  with (f' •ε f'') in X.
-        eapply subst_Ltrans' in vσ.
-        unshelve eapply irrelevanceSubst.
-        -- exists (VPack_Ltrans f'' VΓ).
-           now eapply  WfC_Ltrans.
-        -- now eapply wfc_Ltrans.
-        -- assumption.
-      * pose (i := @in_here_l wl' n false).
-        pose (f' := @LCon_le_up wl wl' n false ne notin f). 
-        pose (f'':= @LCon_le_step wl wl n false ne (wfLCon_le_id _)).
-        pose (f''':= @LCon_le_step wl' wl' n false notin (wfLCon_le_id _)).
-        unshelve eapply VAf ; tea.
-        2: unshelve epose proof (X:= subst_Ltrans f''' _ vσ).
-        1,2: now eapply wfc_Ltrans.
-        change (f''' •ε f)  with (f' •ε f'') in X.
-        eapply subst_Ltrans' in vσ.
-        unshelve eapply irrelevanceSubst.
-        -- exists (VPack_Ltrans f'' VΓ).
-           now eapply  WfC_Ltrans.
-        -- now eapply wfc_Ltrans.
-        -- assumption.
+      intros m.
+      pose (i := @in_here_l wl' n m).
+      pose (f' := @LCon_le_up wl wl' n m ne notin f). 
+      pose (f'':= @LCon_le_step wl wl n m ne (wfLCon_le_id _)).
+      pose (f''':= @LCon_le_step wl' wl' n m notin (wfLCon_le_id _)).
+      unshelve eapply VAt ; tea.
+      2: unshelve epose proof (X:= subst_Ltrans f''' _ vσ).
+      1,2: now eapply wfc_Ltrans.
+      change (f''' •ε f)  with (f' •ε f'') in X.
+      eapply subst_Ltrans' in vσ.
+      unshelve eapply irrelevanceSubst.
+      -- exists (VPack_Ltrans f'' VΓ).
+         now eapply  WfC_Ltrans.
+      -- now eapply wfc_Ltrans.
+      -- assumption.
   - cbn.
     intros.
-    destruct (decidInLCon wl' n) as [ i | i | notin] ; cbn in *.
+    destruct (decidInLCon wl' n) as [ m i | notin] ; cbn in *.
     + pose (f' := LCon_le_in_LCon (ne := ne) f i).
-      pose (f'':= @LCon_le_step wl wl n true ne (wfLCon_le_id _)).
-      unshelve eapply VAextt.
+      pose (f'':= @LCon_le_step wl wl n m ne (wfLCon_le_id _)).
+      unshelve eapply VAt.
       * change f with (f' •ε f'') in vσ'.
         eapply subst_Ltrans' in vσ'.
         unshelve eapply irrelevanceSubst ; [ | assumption | ]. 
         1: now eapply  WfC_Ltrans.
-        exact vσ'.
-      * change f with (f' •ε f'') in vσσ'.
-        unshelve eapply eqsubst_Ltrans' in vσσ'.
-        unshelve eapply irrelevanceSubstEq ; [ | assumption | | ]. 
-        1: now eapply  WfC_Ltrans.
-        2: exact vσσ'.
-    + pose (f' := LCon_le_in_LCon (ne := ne) f i).
-      pose (f'':= @LCon_le_step wl wl n false ne (wfLCon_le_id _)).
-      unshelve eapply VAextf.
-      * change f with (f' •ε f'') in vσ'.
-        eapply subst_Ltrans' in vσ'.
-        unshelve eapply irrelevanceSubst ; [ | assumption | ]. 
-        1: now eapply WfC_Ltrans.
         exact vσ'.
       * change f with (f' •ε f'') in vσσ'.
         unshelve eapply eqsubst_Ltrans' in vσσ'.
@@ -101,83 +63,54 @@ Proof.
         1: now eapply  WfC_Ltrans.
         2: exact vσσ'.
     + unshelve eapply EqSplit.
-      * pose (i := @in_here_l wl' n true).
-        pose (f' := @LCon_le_up wl wl' n true ne notin f). 
-        pose (f'':= @LCon_le_step wl wl n true ne (wfLCon_le_id _)).
-        pose (f''':= @LCon_le_step wl' wl' n true notin (wfLCon_le_id _)).
-        unshelve eapply VAextt ; tea.
-        -- unshelve epose proof (X:= subst_Ltrans f''' _ vσ').
-           1: now eapply wfc_Ltrans.
-           change (f''' •ε f)  with (f' •ε f'') in X.
-           eapply subst_Ltrans' in X.
-           unshelve eapply irrelevanceSubst.
-           ++ exists (VPack_Ltrans f'' VΓ).
-              now eapply  WfC_Ltrans.
-           ++ now eapply wfc_Ltrans.
-           ++ assumption.
-        -- unshelve epose proof (X:= eqsubst_Ltrans f''' _ _ vσσ').
-           1: now eapply wfc_Ltrans.
-           change (f''' •ε f)  with (f' •ε f'') in X.
-           eapply eqsubst_Ltrans' in X.
-           unshelve eapply irrelevanceSubstEq.
-           1: cbn ; exists (VPack_Ltrans f'' VΓ) ; now eapply  WfC_Ltrans.
-           1:  now eapply wfc_Ltrans.
-           2: eassumption.
-      * pose (i := @in_here_l wl' n false).
-        pose (f' := @LCon_le_up wl wl' n false ne notin f). 
-        pose (f'':= @LCon_le_step wl wl n false ne (wfLCon_le_id _)).
-        pose (f''':= @LCon_le_step wl' wl' n false notin (wfLCon_le_id _)).
-        unshelve eapply VAextf ; tea.
-        -- unshelve epose proof (X:= subst_Ltrans f''' _ vσ').
-           1: now eapply wfc_Ltrans.
-           change (f''' •ε f)  with (f' •ε f'') in X.
-           eapply subst_Ltrans' in X.
-           unshelve eapply irrelevanceSubst.
-           ++ exists (VPack_Ltrans f'' VΓ).
-              now eapply  WfC_Ltrans.
-           ++ now eapply wfc_Ltrans.
-           ++ assumption.
-        -- unshelve epose proof (X:= eqsubst_Ltrans f''' _ _ vσσ').
-           1: now eapply wfc_Ltrans.
-           change (f''' •ε f)  with (f' •ε f'') in X.
-           eapply eqsubst_Ltrans' in X.
-           unshelve eapply irrelevanceSubstEq.
-           1: cbn ; exists (VPack_Ltrans f'' VΓ) ; now eapply  WfC_Ltrans.
-           1:  now eapply wfc_Ltrans.
-           2: eassumption.
+      intros m.
+      pose (i := @in_here_l wl' n m).
+      pose (f' := @LCon_le_up wl wl' n m ne notin f). 
+      pose (f'':= @LCon_le_step wl wl n m ne (wfLCon_le_id _)).
+      pose (f''':= @LCon_le_step wl' wl' n m notin (wfLCon_le_id _)).
+      unshelve eapply VAt ; tea.
+      * unshelve epose proof (X:= subst_Ltrans f''' _ vσ').
+        1: now eapply wfc_Ltrans.
+        change (f''' •ε f)  with (f' •ε f'') in X.
+        eapply subst_Ltrans' in X.
+        unshelve eapply irrelevanceSubst.
+        -- exists (VPack_Ltrans f'' VΓ).
+           now eapply  WfC_Ltrans.
+        -- now eapply wfc_Ltrans.
+        -- assumption.
+      * unshelve epose proof (X:= eqsubst_Ltrans f''' _ _ vσσ').
+        1: now eapply wfc_Ltrans.
+        change (f''' •ε f)  with (f' •ε f'') in X.
+        eapply eqsubst_Ltrans' in X.
+        unshelve eapply irrelevanceSubstEq.
+        1: cbn ; exists (VPack_Ltrans f'' VΓ) ; now eapply  WfC_Ltrans.
+        1:  now eapply wfc_Ltrans.
+        2: eassumption.
 Defined.
 
 
 Lemma validEqTySplit {wl : wfLCon} {Γ l A B} {n : nat} {ne : not_in_LCon wl n}
-  {VΓt : [||-v Γ ]< (wl ,,l (ne, true)) >}
-  {VΓf : [||-v Γ ]< (wl ,,l (ne, false)) >}
+  {VΓt : forall m, [||-v Γ ]< (wl ,,l (ne, m)) >}
   {VΓ : [||-v Γ]< wl >}
-  {VAt : [Γ ||-v<l> A | VΓt]< wl ,,l (ne, true) >}
-  {VAf : [Γ ||-v<l> A | VΓf]< wl ,,l (ne, false) >} :
-  [Γ ||-v<l> A ≅ B | VΓt | VAt]< _ > ->
-  [Γ ||-v<l> A ≅ B | VΓf | VAf]< _ > ->
-  [Γ ||-v<l> A ≅ B | VΓ | validTySplit VAt VAf]< wl >.
+  {VAt : forall m, [Γ ||-v<l> A | VΓt m]< wl ,,l (ne, m) >} :
+  (forall m, [Γ ||-v<l> A ≅ B | VΓt m | VAt m]< _ >) ->
+  [Γ ||-v<l> A ≅ B | VΓ | validTySplit VAt]< wl >.
 Proof.
-  intros [VBt] [VBf].
+  intros VBt.
   unshelve econstructor.
   - intros ?????? ; cbn.
-    destruct (decidInLCon wl' n) as [ i | i | notin].
+    destruct (decidInLCon wl' n) as [ m i | notin].
     + now eapply VBt.
-    + now eapply VBf.
     + eapply EqSplit.
-      * now eapply VBt.
-      * now eapply VBf.
+      * intros m ; now eapply VBt.
 Qed.
 
 Lemma validEqTySplit' {wl : wfLCon} {Γ l A B} {n : nat} {ne : not_in_LCon wl n}
-  {VΓt : [||-v Γ ]< (wl ,,l (ne, true)) >}
-  {VΓf : [||-v Γ ]< (wl ,,l (ne, false)) >}
+  {VΓt : forall m, [||-v Γ ]< (wl ,,l (ne, m)) >}
   {VΓ : [||-v Γ]< wl >}
-  {VAt : [Γ ||-v<l> A | VΓt]< wl ,,l (ne, true) >}
-  {VAf : [Γ ||-v<l> A | VΓf]< wl ,,l (ne, false) >}
+  {VAt : forall m, [Γ ||-v<l> A | VΓt m]< wl ,,l (ne, m) >}
   {VA : [Γ ||-v<l> A | VΓ]< wl >}:
-  [Γ ||-v<l> A ≅ B | VΓt | VAt]< _ > ->
-  [Γ ||-v<l> A ≅ B | VΓf | VAf]< _ > ->
+  (forall m, [Γ ||-v<l> A ≅ B | VΓt m | VAt m]< _ >) ->
   [Γ ||-v<l> A ≅ B | VΓ | VA ]< wl >.
 Proof.
   intros.
@@ -186,42 +119,24 @@ Proof.
 Qed.  
 
 Lemma validTmSplit {wl : wfLCon} {Γ l A t} {n : nat} {ne : not_in_LCon wl n}
-  {VΓt : [||-v Γ ]< (wl ,,l (ne, true)) >}
-  {VΓf : [||-v Γ ]< (wl ,,l (ne, false)) >}
+  {VΓt : forall m, [||-v Γ ]< (wl ,,l (ne, m)) >}
   {VΓ : [||-v Γ]< wl >}
-  {VAt : [Γ ||-v<l> A | VΓt]< wl ,,l (ne, true) >}
-  {VAf : [Γ ||-v<l> A | VΓf]< wl ,,l (ne, false) >} :
-  [Γ ||-v<l> t : A | VΓt | VAt]< _ > ->
-  [Γ ||-v<l> t : A | VΓf | VAf]< _ > ->
-  [Γ ||-v<l> t : A | VΓ | validTySplit VAt VAf]< wl >.
+  {VAt : forall m, [Γ ||-v<l> A | VΓt m]< wl ,,l (ne, m) >} :
+  (forall m, [Γ ||-v<l> t : A | VΓt m | VAt m]< _ >) ->
+  [Γ ||-v<l> t : A | VΓ | validTySplit VAt]< wl >.
 Proof.
-  intros [Vtt Vtextt] [Vtf Vtextf].
+  intros Vtt.
   unshelve econstructor.
   - intros ?????? ; cbn.
-    destruct (decidInLCon wl' n) as [ i | i | notin].
+    destruct (decidInLCon wl' n) as [ i | notin].
     + now eapply Vtt.
-    + now eapply Vtf.
     + eapply TmSplit.
-      * now eapply Vtt.
-      * now eapply Vtf.
+      * intros m ; now eapply Vtt.
   - intros ; cbn.
-    destruct (decidInLCon wl' n) as [ i | i | notin].
+    destruct (decidInLCon wl' n) as [ m i | notin].
     + pose (f' := LCon_le_in_LCon (ne := ne) f i).
-      pose (f'':= @LCon_le_step wl wl n true ne (wfLCon_le_id _)).
-      unshelve eapply Vtextt.
-      * change f with (f' •ε f'') in Vσ'.
-        eapply subst_Ltrans' in Vσ'.
-        unshelve eapply irrelevanceSubst ; [ | assumption | ]. 
-        1: now eapply  WfC_Ltrans.
-        exact Vσ'.
-      * change f with (f' •ε f'') in Vσσ'.
-        unshelve eapply eqsubst_Ltrans' in Vσσ'.
-        unshelve eapply irrelevanceSubstEq ; [ | assumption | | ]. 
-        1: now eapply  WfC_Ltrans.
-        2: exact Vσσ'.
-    + pose (f' := LCon_le_in_LCon (ne := ne) f i).
-      pose (f'':= @LCon_le_step wl wl n false ne (wfLCon_le_id _)).
-      unshelve eapply Vtextf.
+      pose (f'':= @LCon_le_step wl wl n m ne (wfLCon_le_id _)).
+      unshelve eapply Vtt.
       * change f with (f' •ε f'') in Vσ'.
         eapply subst_Ltrans' in Vσ'.
         unshelve eapply irrelevanceSubst ; [ | assumption | ]. 
@@ -233,61 +148,36 @@ Proof.
         1: now eapply  WfC_Ltrans.
         2: exact Vσσ'.
     + unshelve eapply TmEqSplit.
-      * pose (i := @in_here_l wl' n true).
-        pose (f' := @LCon_le_up wl wl' n true ne notin f). 
-        pose (f'':= @LCon_le_step wl wl n true ne (wfLCon_le_id _)).
-        pose (f''':= @LCon_le_step wl' wl' n true notin (wfLCon_le_id _)).
-        unshelve eapply Vtextt ; tea.
-        -- unshelve epose proof (X:= subst_Ltrans f''' _ Vσ').
-           1: now eapply wfc_Ltrans.
-           change (f''' •ε f)  with (f' •ε f'') in X.
-           eapply subst_Ltrans' in X.
-           unshelve eapply irrelevanceSubst.
-           ++ exists (VPack_Ltrans f'' VΓ).
-              now eapply  WfC_Ltrans.
-           ++ now eapply wfc_Ltrans.
-           ++ assumption.
-        -- unshelve epose proof (X:= eqsubst_Ltrans f''' _ _ Vσσ').
-           1: now eapply wfc_Ltrans.
-           change (f''' •ε f)  with (f' •ε f'') in X.
-           eapply eqsubst_Ltrans' in X.
-           unshelve eapply irrelevanceSubstEq.
-           1: cbn ; exists (VPack_Ltrans f'' VΓ) ; now eapply  WfC_Ltrans.
-           1:  now eapply wfc_Ltrans.
-           2: eassumption.
-      * pose (i := @in_here_l wl' n false).
-        pose (f' := @LCon_le_up wl wl' n false ne notin f). 
-        pose (f'':= @LCon_le_step wl wl n false ne (wfLCon_le_id _)).
-        pose (f''':= @LCon_le_step wl' wl' n false notin (wfLCon_le_id _)).
-        unshelve eapply Vtextf ; tea.
-        -- unshelve epose proof (X:= subst_Ltrans f''' _ Vσ').
-           1: now eapply wfc_Ltrans.
-           change (f''' •ε f)  with (f' •ε f'') in X.
-           eapply subst_Ltrans' in X.
-           unshelve eapply irrelevanceSubst.
-           ++ exists (VPack_Ltrans f'' VΓ).
-              now eapply  WfC_Ltrans.
-           ++ now eapply wfc_Ltrans.
-           ++ assumption.
-        -- unshelve epose proof (X:= eqsubst_Ltrans f''' _ _ Vσσ').
-           1: now eapply wfc_Ltrans.
-           change (f''' •ε f)  with (f' •ε f'') in X.
-           eapply eqsubst_Ltrans' in X.
-           unshelve eapply irrelevanceSubstEq.
-           1: cbn ; exists (VPack_Ltrans f'' VΓ) ; now eapply  WfC_Ltrans.
-           1:  now eapply wfc_Ltrans.
-           2: eassumption.
+      intros m ; pose (i := @in_here_l wl' n m).
+      pose (f' := @LCon_le_up wl wl' n m ne notin f). 
+      pose (f'':= @LCon_le_step wl wl n m ne (wfLCon_le_id _)).
+      pose (f''':= @LCon_le_step wl' wl' n m notin (wfLCon_le_id _)).
+      unshelve eapply Vtt ; tea.
+      -- unshelve epose proof (X:= subst_Ltrans f''' _ Vσ').
+         1: now eapply wfc_Ltrans.
+         change (f''' •ε f)  with (f' •ε f'') in X.
+         eapply subst_Ltrans' in X.
+         unshelve eapply irrelevanceSubst.
+         ++ exists (VPack_Ltrans f'' VΓ).
+            now eapply  WfC_Ltrans.
+         ++ now eapply wfc_Ltrans.
+         ++ assumption.
+      -- unshelve epose proof (X:= eqsubst_Ltrans f''' _ _ Vσσ').
+         1: now eapply wfc_Ltrans.
+         change (f''' •ε f)  with (f' •ε f'') in X.
+         eapply eqsubst_Ltrans' in X.
+         unshelve eapply irrelevanceSubstEq.
+         1: cbn ; exists (VPack_Ltrans f'' VΓ) ; now eapply  WfC_Ltrans.
+         1:  now eapply wfc_Ltrans.
+         2: eassumption.
 Qed.
 
 Lemma validTmSplit' {wl : wfLCon} {Γ l A t} {n : nat} {ne : not_in_LCon wl n}
-  {VΓt : [||-v Γ ]< (wl ,,l (ne, true)) >}
-  {VΓf : [||-v Γ ]< (wl ,,l (ne, false)) >}
+  {VΓt : forall m, [||-v Γ ]< (wl ,,l (ne, m)) >}
   {VΓ : [||-v Γ]< wl >}
-  {VAt : [Γ ||-v<l> A | VΓt]< wl ,,l (ne, true) >}
-  {VAf : [Γ ||-v<l> A | VΓf]< wl ,,l (ne, false) >}
+  {VAt : forall m, [Γ ||-v<l> A | VΓt m]< wl ,,l (ne, m) >}
   {VA : [Γ ||-v<l> A | VΓ]< wl >}:
-  [Γ ||-v<l> t : A | VΓt | VAt]< _ > ->
-  [Γ ||-v<l> t : A | VΓf | VAf]< _ > ->
+  (forall m, [Γ ||-v<l> t : A | VΓt m | VAt m]< _ >) ->
   [Γ ||-v<l> t : A | VΓ | VA]< wl >.
 Proof.
   intros.
@@ -296,36 +186,28 @@ Proof.
 Qed.  
 
 Lemma validEqTmSplit {wl : wfLCon} {Γ l t u A} {n : nat} {ne : not_in_LCon wl n}
-  {VΓt : [||-v Γ ]< (wl ,,l (ne, true)) >}
-  {VΓf : [||-v Γ ]< (wl ,,l (ne, false)) >}
+  {VΓt : forall m, [||-v Γ ]< (wl ,,l (ne, m)) >}
   {VΓ : [||-v Γ]< wl >}
-  {VAt : [Γ ||-v<l> A | VΓt]< wl ,,l (ne, true) >}
-  {VAf : [Γ ||-v<l> A | VΓf]< wl ,,l (ne, false) >} :
-  [Γ ||-v<l> t ≅ u : A | VΓt | VAt]< _ > ->
-  [Γ ||-v<l> t ≅ u : A | VΓf | VAf]< _ > ->
-  [Γ ||-v<l> t ≅ u : A | VΓ | validTySplit VAt VAf]< wl >.
+  {VAt : forall m, [Γ ||-v<l> A | VΓt m]< wl ,,l (ne, m) >} :
+  (forall m, [Γ ||-v<l> t ≅ u : A | VΓt m | VAt m]< _ >) ->
+  [Γ ||-v<l> t ≅ u : A | VΓ | validTySplit VAt]< wl >.
 Proof.
-  intros [Vtut] [Vtuf].
+  intros Vtut.
   unshelve econstructor.
   - intros ; cbn.
-    destruct (decidInLCon wl' n) as [ i | i | notin].
+    destruct (decidInLCon wl' n) as [ m i | notin].
     + now eapply Vtut.
-    + now eapply Vtuf.
     + eapply TmEqSplit.
-      * now eapply Vtut.
-      * now eapply Vtuf.
+      * intros m ; now eapply Vtut.
 Qed.
         
 
 Lemma validEqTmSplit' {wl : wfLCon} {Γ l t u A} {n : nat} {ne : not_in_LCon wl n}
-  {VΓt : [||-v Γ ]< (wl ,,l (ne, true)) >}
-  {VΓf : [||-v Γ ]< (wl ,,l (ne, false)) >}
+  {VΓt : forall m, [||-v Γ ]< (wl ,,l (ne, m)) >}
   {VΓ : [||-v Γ]< wl >}
-  {VAt : [Γ ||-v<l> A | VΓt]< wl ,,l (ne, true) >}
-  {VAf : [Γ ||-v<l> A | VΓf]< wl ,,l (ne, false) >}
+  {VAt : forall m, [Γ ||-v<l> A | VΓt m]< wl ,,l (ne, m) >}
   {VA : [Γ ||-v<l> A | VΓ]< wl >}:
-  [Γ ||-v<l> t ≅ u : A | VΓt | VAt]< _ > ->
-  [Γ ||-v<l> t ≅ u : A | VΓf | VAf]< _ > ->
+  (forall m, [Γ ||-v<l> t ≅ u : A | VΓt m | VAt m]< _ >) ->
   [Γ ||-v<l> t ≅ u : A | VΓ | VA]< wl >.
 Proof.
   intros.
@@ -334,27 +216,29 @@ Proof.
 Qed.  
 
 Lemma WfCSplit {wl : wfLCon} {Γ} {n : nat} {ne : not_in_LCon wl n} :
-  [||-v Γ ]< (wl ,,l (ne, true)) > ->
-  [||-v Γ ]< (wl ,,l (ne, false)) > ->
+  (forall m, [||-v Γ ]< (wl ,,l (ne, m)) >) ->
   [||-v Γ ]< wl >.
 Proof.
-  intros VGt VGf.
-  epose (Ht := invValidity VGt).
-  epose (Hf := invValidity VGf).
+  intros VGt.
   induction Γ as [ | A ? ?] ; cbn in *.
   - now eapply validEmpty'.
   - cbn in *.
-    destruct Ht as [lt [VGt' [VAt [Hsubt [Hextt Heqt]]]]].
-    destruct Hf as [lf [VGf' [VAf [Hsubf [Hextf Heqf]]]]].
     unshelve eapply validSnoc'.
-    1: destruct lt ; [destruct lf ; [exact zero | exact one] | exact one].
-    1: now eapply IHΓ.
-    all: cbn.
-    1:{ destruct lt, lf.
-        all: eapply validTySplit ; try eassumption.
-        1,2 : eapply embValidTy ; try eassumption.
-        all: now constructor.
+    1: exact one.
+    1:{ eapply IHΓ.
+        intros m.
+        exact (projT1 (projT2 (invValidity (VGt m)))).
     }
+    unshelve eapply validTySplit ; [ | eassumption | ..] ; intros m.
+    1: exact (projT1 (projT2 (invValidity (VGt m)))).
+    destruct (invValidity (VGt m)) as [lt [VGt' [VAt [Hsubt [Hextt Heqt]]]]].
+    destruct lt.
+    + eapply embValidTy ; try eassumption.
+      1: now constructor.
+      eapply irrelevanceTy.
+      exact VAt.
+    + eapply irrelevanceTy.
+      exact VAt.
 Qed.
 
 End Split.
